cedar-lean/Cedar/Thm/Validation/Levels.lean
@@ -37,12 +37,13 @@ open Cedar.Data
 open Cedar.Spec
 open Cedar.Validation
 
-theorem level_based_slicing_is_sound_expr {e : Expr} {n : Nat} {tx : TypedExpr} {c c₁ : Capabilities} {env : Environment} {request : Request} {entities slice : Entities}
-  (hs : slice = entities.sliceAtLevel request n)
+theorem level_based_slicing_is_sound_expr {e : Expr} {n nmax : Nat} {tx : TypedExpr} {c c₁ : Capabilities} {env : Environment} {request : Request} {entities slice : Entities}
+  (hn : nmax ≥ n)
+  (hs : slice = entities.sliceAtLevel request nmax)
   (hc : CapabilitiesInvariant c request entities)
   (hr : RequestAndEntitiesMatchEnvironment env request entities)
   (ht : typeOf e c env = Except.ok (tx, c₁))
-  (hl : TypedExpr.AtLevel tx n) :
+  (hl : TypedExpr.AtLevel tx n nmax) :
   evaluate e request entities = evaluate e request slice
 := by
   cases e
@@ -52,28 +53,28 @@ theorem level_based_slicing_is_sound_expr {e : Expr} {n : Nat} {tx : TypedExpr} 
     have ihc := @level_based_slicing_is_sound_expr c
     have iht := @level_based_slicing_is_sound_expr t
     have ihe := @level_based_slicing_is_sound_expr e
-    exact level_based_slicing_is_sound_if hs hc hr ht hl ihc iht ihe
+    exact level_based_slicing_is_sound_if hn hs hc hr ht hl ihc iht ihe
   case and e₁ e₂ =>
     have ih₁ := @level_based_slicing_is_sound_expr e₁
     have ih₂ := @level_based_slicing_is_sound_expr e₂
-    exact level_based_slicing_is_sound_and hs hc hr ht hl ih₁ ih₂
+    exact level_based_slicing_is_sound_and hn hs hc hr ht hl ih₁ ih₂
   case or e₁ e₂ =>
     have ih₁ := @level_based_slicing_is_sound_expr e₁
     have ih₂ := @level_based_slicing_is_sound_expr e₂
-    exact level_based_slicing_is_sound_or hs hc hr ht hl ih₁ ih₂
+    exact level_based_slicing_is_sound_or hn hs hc hr ht hl ih₁ ih₂
   case unaryApp op e =>
     have ihe := @level_based_slicing_is_sound_expr e
-    exact level_based_slicing_is_sound_unary_app hs hc hr ht hl ihe
+    exact level_based_slicing_is_sound_unary_app hn hs hc hr ht hl ihe
   case binaryApp op e₁ e₂ =>
     have ihe₁ := @level_based_slicing_is_sound_expr e₁
     have ihe₂ := @level_based_slicing_is_sound_expr e₂
-    exact level_based_slicing_is_sound_binary_app hs hc hr ht hl ihe₁ ihe₂
+    exact level_based_slicing_is_sound_binary_app hn hs hc hr ht hl ihe₁ ihe₂
   case getAttr e _ =>
     have ihe := @level_based_slicing_is_sound_expr e
-    exact level_based_slicing_is_sound_get_attr hs hc hr ht hl ihe
+    exact level_based_slicing_is_sound_get_attr hn hs hc hr ht hl ihe
   case hasAttr e _ =>
     have ihe := @level_based_slicing_is_sound_expr e
-    exact level_based_slicing_is_sound_has_attr hs hc hr ht hl ihe
+    exact level_based_slicing_is_sound_has_attr hn hs hc hr ht hl ihe
   case set xs =>
     replace ⟨ hc, txs, ty,  htx, ht ⟩  := type_of_set_inversion ht
     subst tx
@@ -92,7 +93,7 @@ theorem level_based_slicing_is_sound_expr {e : Expr} {n : Nat} {tx : TypedExpr} 
         simp only [Expr.record.sizeOf_spec]
         omega
       exact @level_based_slicing_is_sound_expr x.snd
-    exact level_based_slicing_is_sound_record hs hc hr ht hl ih
+    exact level_based_slicing_is_sound_record hn hs hc hr ht hl ih
 termination_by e
 
 theorem level_based_slicing_is_sound {p : Policy} {n : Nat} {env : Environment} {request : Request} {entities slice : Entities}
@@ -108,4 +109,4 @@ theorem level_based_slicing_is_sound {p : Policy} {n : Nat} {env : Environment} 
   )
   rw [←level_spec] at htl
   have hc := empty_capabilities_invariant request entities
-  exact level_based_slicing_is_sound_expr hs hc hr ht htl
+  exact level_based_slicing_is_sound_expr (by omega) hs hc hr ht htl
